examples/riscv/chacha/chacha_diagonal_round_propScript.sml
@@ -1,0 +1,117 @@
+open HolKernel boolLib Parse bossLib;
+
+open markerTheory wordsTheory wordsLib;
+
+open addressTheory;
+
+open holba_auxiliaryTheory;
+
+open bir_programSyntax bir_program_labelsTheory;
+open bir_immTheory bir_valuesTheory bir_expTheory bir_exp_immTheory;
+open bir_tsTheory bir_bool_expTheory bir_programTheory;
+
+open bir_riscv_backlifterTheory;
+open bir_backlifterLib;
+open bir_compositionLib;
+
+open bir_lifting_machinesTheory;
+open bir_typing_expTheory;
+open bir_htTheory;
+
+open birs_auxTheory;
+
+open total_program_logicTheory;
+open total_ext_program_logicTheory;
+
+open jgmt_rel_bir_contTheory;
+
+open pred_setTheory;
+
+open program_logicSimps;
+
+open bir_env_oldTheory;
+open bir_program_varsTheory;
+
+open HolBACoreSimps;
+
+open chachaTheory;
+open chacha_specTheory;
+open chacha_symb_transf_diagonal_roundTheory;
+
+val _ = new_theory "chacha_diagonal_round_prop";
+
+(* ------------------------------------- *)
+(* Connecting RISC-V and BSPEC contracts *)
+(* ------------------------------------- *)
+
+Theorem chacha_diagonal_round_riscv_pre_imp_bspec_pre_thm:
+ bir_pre_riscv_to_bir
+  (riscv_chacha_diagonal_round_pre pre_arr_0 pre_arr_1 pre_arr_2 pre_arr_3 pre_arr_4 pre_arr_5 pre_arr_6
+    pre_arr_7 pre_arr_8 pre_arr_9 pre_arr_10 pre_arr_11 pre_arr_12 pre_arr_13 pre_arr_14 pre_arr_15)
+  (bspec_chacha_diagonal_round_pre pre_arr_0 pre_arr_1 pre_arr_2 pre_arr_3 pre_arr_4 pre_arr_5 pre_arr_6
+    pre_arr_7 pre_arr_8 pre_arr_9 pre_arr_10 pre_arr_11 pre_arr_12 pre_arr_13 pre_arr_14 pre_arr_15)
+Proof 
+ rw [bir_pre_riscv_to_bir_def,riscv_chacha_diagonal_round_pre_def,bspec_chacha_diagonal_round_pre_def] >-
+  (rw [bir_is_bool_exp_REWRS,bir_is_bool_exp_env_REWRS] >>
+   FULL_SIMP_TAC (std_ss++holBACore_ss) [bir_typing_expTheory.type_of_bir_exp_def]) >>
+ FULL_SIMP_TAC (std_ss++holBACore_ss) [
+  riscv_bmr_rel_EVAL,bir_val_TF_bool2b_DEF,
+  bool2b_def,
+  bool2w_def,
+  w2w_n2w_w2n_64_32
+ ] >>
+ EVAL_TAC
+QED
+
+Theorem chacha_diagonal_round_riscv_post_imp_bspec_post_thm:
+ !ls. bir_post_bir_to_riscv
+   (riscv_chacha_diagonal_round_post pre_arr_0 pre_arr_1 pre_arr_2 pre_arr_3 pre_arr_4 pre_arr_5 pre_arr_6
+     pre_arr_7 pre_arr_8 pre_arr_9 pre_arr_10 pre_arr_11 pre_arr_12 pre_arr_13 pre_arr_14 pre_arr_15)
+   (\l. (bspec_chacha_diagonal_round_post pre_arr_0 pre_arr_1 pre_arr_2 pre_arr_3 pre_arr_4 pre_arr_5 pre_arr_6
+          pre_arr_7 pre_arr_8 pre_arr_9 pre_arr_10 pre_arr_11 pre_arr_12 pre_arr_13 pre_arr_14 pre_arr_15))
+   ls
+Proof
+ cheat
+QED
+
+(* --------------------- *)
+(* Auxiliary definitions *)
+(* --------------------- *)
+
+val progbin_tm = (fst o dest_eq o concl) bir_chacha_progbin_def;
+val riscv_pre_tm = (fst o dest_comb o lhs o snd o strip_forall o concl) riscv_chacha_diagonal_round_pre_def;
+val riscv_post_tm = (fst o dest_comb o lhs o snd o strip_forall o concl) riscv_chacha_diagonal_round_post_def;
+
+(* ---------------------------------- *)
+(* Backlifting BIR contract to RISC-V *)
+(* ---------------------------------- *)
+
+val riscv_cont_chacha_diagonal_round_thm =
+ get_riscv_contract
+  bspec_cont_chacha_diagonal_round
+  progbin_tm riscv_pre_tm riscv_post_tm
+  bir_chacha_prog_def
+  [bspec_chacha_diagonal_round_pre_def]
+  bspec_chacha_diagonal_round_pre_def chacha_diagonal_round_riscv_pre_imp_bspec_pre_thm
+  [bspec_chacha_diagonal_round_post_def] chacha_diagonal_round_riscv_post_imp_bspec_post_thm
+  bir_chacha_riscv_lift_THM;
+
+Theorem riscv_cont_chacha_diagonal_round:
+ riscv_cont bir_chacha_progbin chacha_diagonal_round_init_addr {chacha_diagonal_round_end_addr}
+ (riscv_chacha_diagonal_round_pre pre_arr_0 pre_arr_1 pre_arr_2 pre_arr_3 pre_arr_4 pre_arr_5 pre_arr_6
+   pre_arr_7 pre_arr_8 pre_arr_9 pre_arr_10 pre_arr_11 pre_arr_12 pre_arr_13 pre_arr_14 pre_arr_15)
+ (riscv_chacha_diagonal_round_post pre_arr_0 pre_arr_1 pre_arr_2 pre_arr_3 pre_arr_4 pre_arr_5 pre_arr_6
+   pre_arr_7 pre_arr_8 pre_arr_9 pre_arr_10 pre_arr_11 pre_arr_12 pre_arr_13 pre_arr_14 pre_arr_15)
+Proof
+ rw [chacha_diagonal_round_init_addr_def,chacha_diagonal_round_end_addr_def] >>
+ ACCEPT_TAC riscv_cont_chacha_diagonal_round_thm
+QED
+
+(* ------------------------ *)
+(* Unfolded RISC-V contract *)
+(* ------------------------ *)
+
+val readable_thm = computeLib.RESTR_EVAL_RULE [``riscv_weak_trs``] riscv_cont_chacha_diagonal_round;
+Theorem riscv_cont_chacha_diagonal_round_full = GEN_ALL readable_thm;
+
+val _ = export_theory ();
